\documentclass{article}
\usepackage[a4paper]{geometry}
\usepackage{amsmath}
\usepackage{amssymb}
\usepackage{luatexko}
\usepackage{parskip}
\usepackage{svg}
\usepackage{enumitem}

\setlist[enumerate,1]{label=(\alph*)}

\setmainhangulfont{Nanum Myeongjo}
\setsanshangulfont{Nanum Gothic}

\title{과제7 : 8장 연습문제}
\author{성용운 2017-19937}
\date{}

\begin{document}

\maketitle

\section*{Problem 1}

\begin{align*}
	\sum \widehat{e_i}
	&= \sum (y_i - \widehat{y_i}) \\
	&= \sum \left(\left(y_i - \bar{y}\right) - \widehat{\beta}\left(x_i - \bar{x}\right)\right) \\
	&= \sum (0 - \widehat{\beta} 0) \\
	&= 0 \\
	\sum x_i \widehat{e_i}
	&= \sum x_i \left(y_i - \bar{y} - \widehat{\beta}\left(x_i - \bar{x}\right)\right) \\
	&= \sum \left(x_i y_i -\bar{y}  x_i - \widehat{\beta} \left(x_i^2 - x_i \bar{x}\right)\right) \\
	&= \sum x_i y_i - n\bar{x}\bar{y} - \frac{S_{xy}}{S_{xx}} \sum \left(x_i^2 - x_i \bar{x}\right) \\
	&= \sum x_i y_i - n\bar{x}\bar{y} - \frac{\sum (x_i - \bar{x})(y_i - \bar{y})}{\sum (x_i-\bar{x})^2} \left(\sum x_i^2 - n\bar{x}^2\right) \\
	&= \sum x_i y_i - n\bar{x}\bar{y} - \frac{\sum x_i y_i - n\bar{x}\bar{y}}{\sum x_i^2 -n \bar{x}^2}  \left(\sum x_i^2 - n\bar{x}^2\right) \\
	&= \sum x_i y_i - n\bar{x}\bar{y} - \left(\sum x_i y_i - n\bar{x}\bar{y}\right) \\
	&= 0
\end{align*}

\section*{Problem 2}

\begin{align*}
	2\sum \widehat{e_i} \widehat{\beta} (x_i - \bar{x})
	&= 2\widehat{\beta} \sum (\widehat{e_i} x_i - \widehat{e_i} \bar{x}) \\
	&= 2\widehat{\beta} (0 - 0 \cdot n \bar{x}) \\
	&= 0 \\
	\sum (y_i - \bar{y})^2
	&= \sum ((y_i - \widehat{y_i}) + (\widehat{y_i} - \bar{y}))^2 \\
	&= \sum \left(\left(y_i - \widehat{y_i}\right)^2 + \left(\widehat{y_i} - \bar{y}\right)^2 + 2\left(y_i - \widehat{y_i}\right)\left(\widehat{y_i} - \bar{y}\right)\right) \\
	&= \sum \left(\left(y_i - \widehat{y_i}\right)^2 + \left(\widehat{y_i} - \bar{y}\right)^2\right) \\
	&= \sum (y_i - \widehat{y_i})^2 + \sum (\widehat{y_i} - \bar{y})^2
\end{align*}

\section*{Problem 3}

\begin{align*}
	\sum (\widehat{y_i} - \bar{y})^2
	&= \sum (\widehat{y_i}^2 - 2 \widehat{y_i}\bar{y}) + n\bar{y}^2\\
	&= \sum \widehat{y_i}^2
	- 2 \bar{y} \sum \widehat{y_i}
	+ n\bar{y}^2 \\
	&= 2 n \bar{y}^2
	+ \widehat{\beta}^2 \sum (x_i - \bar{x})^2
	+ 2 \bar{y}\widehat{\beta} \sum (x_i - \bar{x})
	- 2 \bar{y} (n\bar{y} + \widehat{\beta} \sum (x_i - \bar{x})) \\
	&= \widehat{\beta}^2 \sum (x_i - \bar{x})^2
	+ 2 \bar{y}\widehat{\beta} \sum (x_i - \bar{x}) - 2 \bar{y} \widehat{\beta} \sum (x_i - \bar{x}) \\
	&= \boxed{\widehat{\beta}^2 S_{xx}} \\
	&= \frac{S_{xy}^2}{S_{xx}} \\
	&= \frac{(\sum (x_i - \bar{x})(y_i - \bar{y}))^2}{S_{xx}} \\
	&= \frac
		{(\sum (y_i (x_i-\bar{x}) + \bar{x}\bar{y} - x_i \bar{y}))^2}
		{S_{xx}} \\
	&= \frac
		{(\sum y_i (x_i-\bar{x}))^2}
		{S_{xx}} \\
	&= \boxed{\left(\sum c_i y_i\right)^2}
\end{align*}

\section*{Problem 4}

\begin{align*}
	\widehat{\beta}^2 S_{xx} &= \frac{(\sum y_i(x_i - \bar{x}))^2}{S_{xx}} \\
	\text{therefore,}\, \widehat{\beta}
	&= \boxed{\sum c_i y_i} \\
	\widehat{\alpha} + \widehat{\beta}x
	&= \bar{y} - \bar{x} \widehat{\beta} + x \widehat{\beta} \\
	&= \bar{y} + (x - \bar{x}) \left(\sum \frac{y_i (x_i - \bar{x})}{S_{xx}}\right) \\
	&= \sum \left(\frac{y_i}{n} + \frac{y_i (x - \bar{x})(x_i - \bar{x})}{S_{xx}}\right) \\
	&= \boxed{\sum d_i y_i}
\end{align*}
\begin{align*}
	E\left(\widehat{\beta}\right)
	&= E\left(\sum c_i y_i \right) \\
	&= \sum c_i E(\alpha + \beta x_i + e_i) \\
	&= \sum c_i (\alpha + \beta x_i) \\
	&= \alpha \sum c_i + \beta \sum c_i x_i \\
	&= \beta \frac{\sum (x_i^2 - x_i \bar{x})}{\sum (x_i - \bar{x})^2} \\
	&= \beta \frac{\sum x_i^2 - n\bar{x}^2}{\sum x_i^2 - n\bar{x}^2} \\
	&= \boxed{\beta}
\end{align*}
\begin{align*}
	\mathrm{Var}\left(\widehat{\beta}\right)
	&= \mathrm{Var}\left(\sum c_i y_i \right) \\
	&= \sum c_i^2 \mathrm{Var}(y_i) \\
	&= \sum c_i^2 \mathrm{Var}(\alpha + \beta x_i + e_i) \\
	&= \sum c_i^2 \mathrm{Var}(e_i) \\
	&= \boxed{\sigma / S_{xx}}
\end{align*}
\begin{align*}
	E\left(\widehat{\alpha} + \widehat{\beta}x\right)
	&= E\left(\bar{y} - \widehat{\beta}\bar{x} + \widehat{\beta}x\right) \\
	&= \boxed{\alpha + \beta x}
\end{align*}
\begin{align*}
	\mathrm{Var}\left(\widehat{\alpha} + \widehat{\beta}x\right)
	&= \mathrm{Var}\left(\sum d_i y_i \right) \\
	&= \sum d_i^2 \mathrm{Var}(y_i) \\
	&= \sum d_i^2 \sigma^2 \\
	&= \sigma^2 \sum \left(\frac{1}{n} + \frac{(x - \bar{x})(x_i - \bar{x})}{S_{xx}}\right)^2 \\
	&= \boxed{\sigma^2 \left(\frac{1}{n} + \frac{(x - \bar{x})^2}{S_{xx}}\right)} \\
\end{align*}

\section*{Problem 5}

\begin{enumerate}
	\item ~ \\ \includesvg{hw07-p05-a-01.svg}
	\item $r = S_{xy}/\sqrt{S_{xx} S_{yy}} = 0.975$
	\item
		\begin{gather*}
			t = \sqrt{n-2} \frac{r}{\sqrt{1-r^2}} = 17.471 \\
			t \ge t_{\alpha}(n-2) = 2.583
		\end{gather*}
		We reject the null hypothesis, there is evidence of correlation
		between these two variables.
\end{enumerate}

\section*{Problem 7}

\begin{center}
\begin{tabular}{c|ccccc}
	요인 & 제곱합 & 자유도 & 평균제곱 & F 값 & 유의확률 \\
	\hline
	회귀 & 18.066 & 1 & 18.066 & 7.987 & 0.022 \\
	잔차 & 18.094 & 8 & 2.262  & \\
	\hline
	계   & 36.16  & 9 \\
\end{tabular}
\end{center}

$R^2 = 0.500$, $\widehat{\sigma} = 1.504$

We fail to reject the null hypothesis, as $P(F \ge f) = 0.022 \ge 0.01$. There
is not enough evidence to suggest that these two variables are linearly
related.

\section*{Problem 8}

\begin{itemize}
	\item With outlier: $\widehat{y} = 5.279 + 0.936 x$
	\item With outlier removed: $\widehat{y} = 5.702 + 0.936 x$
\end{itemize}

\begin{center}
\begin{tabular}{c|ccccc}
	요인 & 제곱합 & 자유도 & 평균제곱 & F 값 & 유의확률 \\
	\hline
	회귀 & 18.066 & 1 & 18.066 & 61.692 & 0.0001 \\
	잔차 & 2.05   & 7 & 0.293  & \\
	\hline
	계   & 20.116 & 8 \\
\end{tabular}
\end{center}

$R^2 = 0.898$.

We reject the null hypothesis, as $P(F \ge f) = 0.0001 \le 0.01$. There is
evidence to suggest that these two variables are linearly related.

\end{document}
